commit

AP/System/Symmetry/Defs.lean
@@ -1,107 +1,107 @@
-import AP.System.Symmetry.Raw0
+import AP.System.Symmetry.Raw
 
-namespace System.Symmetry
+namespace System
 
 universe u
 variable {S T : Type u} {sys : System S T}
 
-structure Raw (sys : System S T) : Type u extends Raw₀ sys where
-  wf : toRaw₀.WF
+structure Symmetry (sys : System S T) : Type u extends Raw sys where
+  wf : toRaw.WF
 
-namespace Raw
+namespace Symmetry
 
-variable {sym sym₁ sym₂ sym₃ : Raw sys}
+variable {sym sym₁ sym₂ sym₃ : Symmetry sys}
 
 @[ext]
-theorem ext (h : sym₁.toRaw₀ = sym₂.toRaw₀) : sym₁ = sym₂ := by
+theorem ext (h : sym₁.toRaw = sym₂.toRaw) : sym₁ = sym₂ := by
   cases sym₁; cases sym₂; simp_all
 
-def one : Raw sys :=
-  ⟨Raw₀.one, inferInstance⟩
+def one : Symmetry sys :=
+  ⟨Raw.one, inferInstance⟩
 
-instance : Inhabited (Raw sys) := ⟨one⟩
-theorem default_eq : (default : Raw sys) = one := rfl
+instance : Inhabited (Symmetry sys) := ⟨one⟩
+theorem default_eq : (default : Symmetry sys) = one := rfl
 
-instance : sym.toRaw₀.WF := sym.wf
+instance : sym.toRaw.WF := sym.wf
 
 theorem tr_fs {s t} [hs : sys.WF s] :
-sys.tr (sym.fs s) t = (sys.tr s (sym.ft' t)).map sym.fs := Raw₀.tr_fs
+sys.tr (sym.fs s) t = (sys.tr s (sym.ft' t)).map sym.fs := Raw.tr_fs
 
 theorem tr_fs' {s t} [hs : sys.WF s] :
-sys.tr (sym.fs' s) t = (sys.tr s (sym.ft t)).map sym.fs' := Raw₀.tr_fs'
+sys.tr (sym.fs' s) t = (sys.tr s (sym.ft t)).map sym.fs' := Raw.tr_fs'
 
 theorem tr_ft {s t} [hs : sys.WF s] :
-sys.tr s (sym.ft t) = (sys.tr (sym.fs' s) t).map sym.fs := Raw₀.tr_ft
+sys.tr s (sym.ft t) = (sys.tr (sym.fs' s) t).map sym.fs := Raw.tr_ft
 
 theorem tr_ft' {s t} [hs : sys.WF s] :
-sys.tr s (sym.ft' t) = (sys.tr (sym.fs s) t).map sym.fs' := Raw₀.tr_ft'
+sys.tr s (sym.ft' t) = (sys.tr (sym.fs s) t).map sym.fs' := Raw.tr_ft'
 
 theorem validTr_fs_of {s t} [hs : sys.WF s]
-(h : sys.validTr s (sym.ft' t)) : sys.validTr (sym.fs s) t := Raw₀.validTr_fs_of h
+(h : sys.validTr s (sym.ft' t)) : sys.validTr (sym.fs s) t := Raw.validTr_fs_of h
 
 theorem validTr_fs'_of {s t} [hs : sys.WF s]
-(h : sys.validTr s (sym.ft t)) : sys.validTr (sym.fs' s) t := Raw₀.validTr_fs'_of h
+(h : sys.validTr s (sym.ft t)) : sys.validTr (sym.fs' s) t := Raw.validTr_fs'_of h
 
 theorem validTr_ft_of {s t} [hs : sys.WF s]
-(h : sys.validTr (sym.fs' s) t) : sys.validTr s (sym.ft t) := Raw₀.validTr_ft_of h
+(h : sys.validTr (sym.fs' s) t) : sys.validTr s (sym.ft t) := Raw.validTr_ft_of h
 
 theorem validTr_ft'_of {s t} [hs : sys.WF s]
-(h : sys.validTr (sym.fs s) t) : sys.validTr s (sym.ft' t) := Raw₀.validTr_ft'_of h
+(h : sys.validTr (sym.fs s) t) : sys.validTr s (sym.ft' t) := Raw.validTr_ft'_of h
 
 theorem validTr_fs {s t} [hs : sys.WF s] :
-sys.validTr (sym.fs s) t ↔ sys.validTr s (sym.ft' t) := Raw₀.validTr_fs
+sys.validTr (sym.fs s) t ↔ sys.validTr s (sym.ft' t) := Raw.validTr_fs
 
 theorem validTr_fs' {s t} [hs : sys.WF s] :
-sys.validTr (sym.fs' s) t ↔ sys.validTr s (sym.ft t) := Raw₀.validTr_fs'
+sys.validTr (sym.fs' s) t ↔ sys.validTr s (sym.ft t) := Raw.validTr_fs'
 
 theorem validTr_ft {s t} [hs : sys.WF s] :
-sys.validTr s (sym.ft t) ↔ sys.validTr (sym.fs' s) t := Raw₀.validTr_ft
+sys.validTr s (sym.ft t) ↔ sys.validTr (sym.fs' s) t := Raw.validTr_ft
 
 theorem validTr_ft' {s t} [hs : sys.WF s] :
 sys.validTr s (sym.ft' t) ↔ sys.validTr (sym.fs s) t :=
   ⟨validTr_fs_of, validTr_ft'_of⟩
 
-def simFn (sym : Raw sys) (f : S → T) (s : S) : T :=
-  sym.toRaw₀.simFn f s
+def simFn (sym : Symmetry sys) (f : S → T) (s : S) : T :=
+  sym.toRaw.simFn f s
 
 instance {f} [hf : sys.SimFn f] : sys.SimFn (sym.simFn f) := by
   unfold simFn; infer_instance
 
-def inv (sym : Raw sys) : Raw sys :=
-  ⟨sym.toRaw₀.inv, inferInstance⟩
+def inv (sym : Symmetry sys) : Symmetry sys :=
+  ⟨sym.toRaw.inv, inferInstance⟩
 
 @[simp]
-theorem inv_inv : sym.inv.inv = sym := ext Raw₀.inv_inv
+theorem inv_inv : sym.inv.inv = sym := ext Raw.inv_inv
 
-def mul (sym₁ sym₂ : Raw sys) : Raw sys :=
-  ⟨sym₁.toRaw₀.mul sym₂.toRaw₀, inferInstance⟩
+def mul (sym₁ sym₂ : Symmetry sys) : Symmetry sys :=
+  ⟨sym₁.toRaw.mul sym₂.toRaw, inferInstance⟩
 
-def npow (n : ℕ) (sym : Raw sys) : Raw sys :=
-  ⟨sym.toRaw₀.npow n, inferInstance⟩
+def npow (n : ℕ) (sym : Symmetry sys) : Symmetry sys :=
+  ⟨sym.toRaw.npow n, inferInstance⟩
 
-def zpow (z : ℤ) (sym : Raw sys) : Raw sys :=
-  ⟨sym.toRaw₀.zpow z, inferInstance⟩
+def zpow (z : ℤ) (sym : Symmetry sys) : Symmetry sys :=
+  ⟨sym.toRaw.zpow z, inferInstance⟩
 
-def Equiv (sym₁ sym₂ : Raw sys) : Prop :=
-  sym₁.toRaw₀.Equiv sym₂.toRaw₀
+def Equiv (sym₁ sym₂ : Symmetry sys) : Prop :=
+  sym₁.toRaw.Equiv sym₂.toRaw
 
 @[simp, refl]
-theorem Equiv.refl : sym.Equiv sym := Raw₀.Equiv.refl
+theorem Equiv.refl : sym.Equiv sym := Raw.Equiv.refl
 
 @[symm]
 theorem Equiv.symm (h : sym₁.Equiv sym₂) : sym₂.Equiv sym₁ :=
-  Raw₀.Equiv.symm h
+  Raw.Equiv.symm h
 
 @[trans]
 theorem Equiv.trans (h₁ : sym₁.Equiv sym₂) (h₂ : sym₂.Equiv sym₃) : sym₁.Equiv sym₃ :=
-  Raw₀.Equiv.trans h₁ h₂
+  Raw.Equiv.trans h₁ h₂
 
 theorem Equiv.iseqv : Equivalence # Equiv (sys := sys) where
   refl := λ _ => refl
   symm := symm
   trans := trans
 
-instance setoid : Setoid (Raw sys) where
+instance setoid : Setoid (Symmetry sys) where
   r := Equiv
   iseqv := Equiv.iseqv
 
