AP/System/Symmetry.lean
@@ -1,1 +1,1 @@
-import AP.System.Symmetry.Defs
+import AP.System.Symmetry.Basic
