AP/System/Symmetry/Basic.lean
@@ -1,0 +1,3 @@
+import AP.System.Symmetry.Raw
+
+namespace System.Symmetry
